theories/typing/array.v
@@ -1,8 +1,8 @@
 Require Import FunctionalExtensionality Equality.
 From iris.proofmode Require Import tactics.
 From lrust.util Require Import basic types.
-From lrust.typing Require Import product mod_ty.
 From lrust.typing Require Export type.
+From lrust.typing Require Import product mod_ty.
 Set Default Proof Using "Type".
 
 Section array.
